semantics rewriting

Logic/Logic/Kripke/Basic.lean
@@ -1,3 +1,4 @@
+import Logic.Logic.Kripke.RelItr
 import Logic.Logic.Semantics
 import Logic.Logic.System
 import Logic.Vorspiel.BinaryRelations
@@ -19,6 +20,46 @@ instance {F : Frame} : Nonempty F.World := F.World_nonempty
 
 abbrev Frame.Rel' {F : Frame} (x y : F.World) := F.Rel x y
 scoped infix:45 " ≺ " => Frame.Rel'
+
+protected abbrev Frame.RelItr' {F : Frame} (n : ℕ) := F.Rel.iterate n
+scoped notation x:45 " ≺^[" n "] " y:46 => Frame.RelItr' n x y
+
+-- TODO: `Rel.iterate`上で示せるはず
+namespace Frame.RelItr'
+
+lemma congr {F : Frame} {x y : F.World} {n m : ℕ} (h : x ≺^[n] y) (he : n = m := by omega) : x ≺^[m] y := by
+  subst_vars; exact h;
+
+lemma forward {F : Frame} {x y : F.World} : x ≺^[n + 1] y ↔ ∃ z, x ≺^[n] z ∧ z ≺ y := Rel.iterate.forward
+
+lemma comp {F : Frame} {x y : F.World} {n m : ℕ} : (∃ z, x ≺^[n] z ∧ z ≺^[m] y) ↔ x ≺^[n + m] y := by
+  constructor;
+  . rintro ⟨z, hzx, hzy⟩;
+    induction n generalizing x with
+    | zero => simp_all;
+    | succ n ih =>
+      suffices x ≺^[(n + m + 1)] y by apply congr this;
+      obtain ⟨w, hxw, hwz⟩ := hzx;
+      use w;
+      constructor;
+      . exact hxw;
+      . exact @ih w hwz;
+  . rintro h;
+    induction n generalizing x with
+    | zero => simp_all;
+    | succ n ih =>
+      have rxy : x ≺^[n + m + 1] y := congr h;
+      obtain ⟨w, rxw, rwy⟩ := rxy;
+      obtain ⟨u, rwu, ruy⟩ := @ih w rwy;
+      use u;
+      constructor;
+      . use w;
+      . assumption;
+
+lemma comp' {F : Frame} {x y : F.World} {n m : ℕ+} : (∃ z, x ≺^[n] z ∧ z ≺^[m] y) ↔ x ≺^[n + m] y := comp
+
+end Frame.RelItr'
+
 
 noncomputable abbrev Frame.default {F : Frame} : F.World := Classical.choice F.World_nonempty
 notation "﹫" => Frame.default
@@ -130,7 +171,7 @@ abbrev FrameClass.Dep (α : Type v) := FrameClass.{u}
 abbrev FrameClass.alt (𝔽 : FrameClass) (α) : FrameClass.Dep α := 𝔽
 notation 𝔽:max "#" α:max => FrameClass.alt 𝔽 α
 
-/-
+
 abbrev FiniteFrameClass := Set (FiniteFrame)
 
 @[simp] def FiniteFrameClass.toFrameClass (𝔽 : FiniteFrameClass) : FrameClass := { F | ∃ F', F' ∈ 𝔽 ∧ F'.toFrame = F }
@@ -145,15 +186,12 @@ postfix:max "ꟳ" => FrameClass.restrictFinite
 lemma FrameClass.iff_mem_restrictFinite {𝔽 : FrameClass} {F : Frame} (h : F ∈ 𝔽) (F_finite : Finite F.World) : F ∈ 𝔽ꟳ := by
   simp;
   use { toFrame := F, World_finite := F_finite };
--/
 
--- set_option pp.universes true in
-/-
-abbrev FrameClassOfSystem {F : Type u} [System F S] (𝓢 : S) (α : Type u) [Semantics F (Frame.Dep α)] : FrameClass.Dep α := { F | F ⊧* System.theory 𝓢 }
-notation "𝔽(" 𝓢 " of " α ")" => FrameClassOfSystem 𝓢 α
--/
 
 section
+
+/-- FrameClass for `𝐊` -/
+abbrev AllFrameClass : FrameClass := Set.univ
 
 /-- FrameClass for `𝐈𝐧𝐭` and `𝐒𝟒` -/
 abbrev ReflexiveTransitiveFrameClass : FrameClass := λ F => Reflexive F ∧ Transitive F
@@ -174,6 +212,13 @@ class FrameClass.Characteraizable (𝔽₁ : FrameClass) (𝔽₂ : outParam (Fr
   characterize : ∀ {F}, F ∈ 𝔽₂ → F ∈ 𝔽₁
   nonempty : ∃ F, F ∈ 𝔽₂
 
+class FrameClass.DefinedBy (𝔽₁ : FrameClass) (𝔽₂ : outParam (FrameClass)) where
+  define : ∀ {F}, F ∈ 𝔽₁ ↔ F ∈ 𝔽₂
+  nonempty : ∃ F, F ∈ 𝔽₂
+
+instance {𝔽₁ 𝔽₂ : FrameClass} [defines : 𝔽₁.DefinedBy 𝔽₂] : FrameClass.Characteraizable 𝔽₁ 𝔽₂ where
+  characterize hF := defines.define.mpr hF
+  nonempty := defines.nonempty
 
 abbrev Valuation (F : Frame) (α : Type*) := F.World → α → Prop
 
@@ -194,7 +239,6 @@ abbrev ClassicalFrame : Kripke.Frame where
   World := Unit
   Rel _ _ := True
 
-
 namespace ClassicalFrame
 
 @[simp] lemma transitive : Transitive ClassicalFrame := by simp [Transitive];
@@ -211,7 +255,6 @@ namespace ClassicalFrame
 
 end ClassicalFrame
 
-
 abbrev ClassicalValuation (α : Type*) := α → Prop
 
 abbrev ClassicalModel (V : ClassicalValuation α) : Kripke.Model α where
@@ -219,6 +262,31 @@ abbrev ClassicalModel (V : ClassicalValuation α) : Kripke.Model α where
   Valuation _ a := V a
 
 end Classical
+
+
+/-- Frame with single world and identiy relation -/
+abbrev terminalFrame : FiniteFrame where
+  World := Unit;
+  Rel := λ _ _ => True
+
+@[simp]
+lemma terminalFrame.iff_rel' {x y : terminalFrame.World} : x ≺ y ↔ x = y := by
+  simp [Frame.Rel'];
+
+@[simp]
+lemma terminalFrame.iff_relItr' {x y : terminalFrame.World} : x ≺^[n] y ↔ x = y := by
+  induction n with
+  | zero => simp;
+  | succ n ih => simp_all;
+
+
+
+abbrev PointFrame : FiniteFrame where
+  World := Unit
+  Rel := (λ _ _ => False)
+
+@[simp]
+lemma PointFrame.iff_rel' {x y : PointFrame.World} : ¬(x ≺ y) := by simp [Frame.Rel'];
 
 
 end LO.Kripke
