Logic/Logic/Kripke/RelItr.lean
@@ -1,0 +1,41 @@
+import Mathlib.Data.Rel
+
+def Rel.iterate (R : Rel α α) : ℕ → α → α → Prop
+  | 0 => (· = ·)
+  | n + 1 => fun x y ↦ ∃ z, R x z ∧ R.iterate n z y
+
+namespace Rel.iterate
+
+variable {R : Rel α α} {n : ℕ}
+
+@[simp]
+lemma iff_zero {x y : α} : R.iterate 0 x y ↔ x = y := iff_of_eq rfl
+
+@[simp]
+lemma iff_succ {x y : α} : R.iterate (n + 1) x y ↔ ∃ z, R x z ∧ R.iterate n z y := iff_of_eq rfl
+
+@[simp]
+lemma eq : Rel.iterate (α := α) (· = ·) n = (· = ·) := by
+  induction n with
+  | zero => rfl;
+  | succ n ih => aesop
+
+lemma forward : (R.iterate (n + 1) x y) ↔ ∃ z, R.iterate n x z ∧ R z y := by
+  induction n generalizing x y with
+  | zero => simp_all;
+  | succ n ih =>
+    constructor;
+    . rintro ⟨z, Rxz, Rzy⟩;
+      obtain ⟨w, Rzw, Rwy⟩ := ih.mp Rzy;
+      use w;
+      constructor;
+      . use z;
+      . assumption;
+    . rintro ⟨z, ⟨w, Rxw, Rwz⟩, Rzy⟩;
+      use w;
+      constructor;
+      . assumption;
+      . apply ih.mpr;
+        use z;
+
+end Rel.iterate
