Logic/Modal/Standard/Kripke/Completeness.lean
@@ -193,7 +193,7 @@ lemma complete_of_mem_canonicalFrame [Inhabited (Λ)-MCT] {𝔽 : FrameClass.Dep
 lemma instComplete_of_mem_canonicalFrame [Inhabited (Λ)-MCT] {𝔽 : FrameClass.Dep α} (hFC : CanonicalFrame Λ ∈ 𝔽) : Complete (Λ) 𝔽 := ⟨complete_of_mem_canonicalFrame hFC⟩
 
 instance K_complete : Complete (𝐊 : DeductionParameter.{u} α) AllFrameClass.{u}# := by
-  simpa [←Normal.isK] using instComplete_of_mem_canonicalFrame (𝔽 := AllFrameClass#) trivial;
+  simpa [←Normal.K_is_K_normal] using instComplete_of_mem_canonicalFrame (𝔽 := AllFrameClass#) trivial;
 
 end Kripke
 
